import Relation.Binary.PropositionalEquality as Eq
open Eq using (_≡_; refl)
open Eq.≡-Reasoning using (begin_; _≡⟨⟩_; _∎)
module nat where
data ℕ : Set where
  zero : ℕ
  suc  : ℕ → ℕ
{-# BUILTIN NATURAL ℕ #-}
_+_ : ℕ → ℕ → ℕ
zero + n = n
(suc m) + n = suc (m + n)

_ : 2 + 3 ≡ 5
_ = refl

_*_ : ℕ → ℕ → ℕ
zero    * n  =  zero
(suc m) * n  =  n + (m * n)

_^_ : ℕ → ℕ → ℕ
m ^ 0        =  1
m ^ (suc n)  =  m * (m ^ n)

_∸_ : ℕ → ℕ → ℕ
m     ∸ zero   =  m
zero  ∸ suc n  =  zero
suc m ∸ suc n  =  m ∸ n
