import Relation.Binary.PropositionalEquality as Eq
open Eq using (_≡_; refl; cong)
open import Data.Nat using (ℕ; zero; suc; _+_; _*_)
open import Data.Nat.Properties using (+-comm; +-identityʳ; *-comm)
module relations where
data _≤_ : ℕ → ℕ → Set where

  z≤n : ∀ {n : ℕ}
      --------
    → zero ≤ n

  s≤s : ∀ {m n : ℕ}
    → m ≤ n
      -------------
    → suc m ≤ suc n

infix 4 _≤_

≤-refl : ∀ {n : ℕ}
    -----
  → n ≤ n
≤-refl {zero} = z≤n
≤-refl {suc n} = s≤s ≤-refl

≤-trans : ∀ {m n p : ℕ}
  → m ≤ n
  → n ≤ p
    -----
  → m ≤ p
≤-trans z≤n x₁ = z≤n
≤-trans (s≤s x) (s≤s x₁) = s≤s (≤-trans x x₁)

≤-antisym : ∀ {m n : ℕ}
  → n ≤ m
  → m ≤ n
   -------
  → m ≡ n
≤-antisym z≤n z≤n = refl
≤-antisym (s≤s n≤m) (s≤s m≤n) rewrite ≤-antisym n≤m m≤n = refl

data Total (m n : ℕ) : Set where

  forward :
      m ≤ n
      ---------
    → Total m n

  flipped :
      n ≤ m
      ---------
    → Total m n

≤-total : ∀ (m n : ℕ) → Total m n
≤-total zero    n                         =  forward z≤n
≤-total (suc m) zero                      =  flipped z≤n
≤-total (suc m) (suc n) with ≤-total m n
...                        | forward m≤n  =  forward (s≤s m≤n)
...                        | flipped n≤m  =  flipped (s≤s n≤m)

+-monoʳ-≤ : ∀ (n p q : ℕ)
     → p ≤ q
     -------------
     → n + p ≤ n + q
+-monoʳ-≤ zero p q p≤q = p≤q
+-monoʳ-≤ (suc n) p q p≤q = s≤s (+-monoʳ-≤ n p q p≤q)

+-monoˡ-≤ : ∀ (m n p : ℕ)
     → m ≤ n
     -------------
     → m + p ≤ n + p
+-monoˡ-≤ m n p m≤n  rewrite +-comm m p | +-comm n p = +-monoʳ-≤ p m n m≤n

+-mono-≤ : ∀ (m n p q : ℕ)
  → m ≤ n
  → p ≤ q
    -------------
  → m + p ≤ n + q

+-mono-≤ m n p q m≤n p≤q = ≤-trans (+-monoˡ-≤ m n p m≤n) (+-monoʳ-≤ n p q p≤q)

*-monoʳ-≤ : ∀ (n p q : ℕ)
     → p ≤ q
     -------------
     → n * p ≤ n * q

*-monoʳ-≤ zero p q p≤q = z≤n
*-monoʳ-≤ (suc n) p q p≤q = +-mono-≤ p q (n * p) (n * q) p≤q (*-monoʳ-≤ n p q p≤q)

*-monoˡ-≤ : ∀ (m n p : ℕ)
     → m ≤ n
     -------------
     → m * p ≤ n * p
*-monoˡ-≤ m n p m≤n  rewrite *-comm m p | *-comm n p = *-monoʳ-≤ p m n m≤n

*-mono-≤ : ∀ (m n p q : ℕ)
  → m ≤ n
  → p ≤ q
  -------
  → m * p ≤ n * q
*-mono-≤ m n p q m≤n p≤q = ≤-trans (*-monoˡ-≤ m n p m≤n) (*-monoʳ-≤ n p q p≤q)
